Makefile
@@ -53,6 +53,7 @@ OCAMLOPT=ocamlopt
 
 # TODO: rename coq into jscoq
 
+
 JS_SRC=\
 	coq/Shared.v \
 	coq/JsNumber.v \
@@ -62,11 +63,15 @@ JS_SRC=\
 	coq/JsPreliminary.v \
 	coq/JsPreliminaryAux.v \
 	coq/JsInit.v \
+	coq/JsInterpreter.v \
+  coq/JsInterpreterExtraction.v \
 	coq/JsPrettyInterm.v \
 	coq/JsPrettyIntermAux.v \
 	coq/JsPrettyRules.v \
+	coq/JsCorrectness.v \
 	coq/JsWellFormednessDef.v \
 	coq/JsWellFormednessProof.v
+
 
 JS_VO=$(JS_SRC:.v=.vo)
 
